Pom/Linearization/Singleton.lean
@@ -1,0 +1,120 @@
+import Pom.Linearization
+
+open Linearization
+
+namespace Label
+
+def eval {t : Type → Type} {s act test : Type}
+    [Linearizable t s] [Bot (t s)]
+    [Sem act s (t s)] [Sem test s (t Bool)]
+    (ℓ : Label act test) : s → t s :=
+  match ℓ with
+    | Label.bot => ⊥
+    | Label.fork => pure
+    | Label.act a => Sem.sem a
+    | Label.test b => fun σ ↦ (Sem.sem b σ : t Bool) *> pure σ
+
+end Label
+
+namespace Lpofin
+
+lemma singleton_next {l : Type} [Bot l] (x : Node) (ℓ : l) :
+    next (singleton x ℓ) (singleton x ℓ).nodes_finset = {x} := by
+  classical
+  ext y; constructor
+  · intro h; have ⟨hy, _, _⟩ := Finset.mem_filter.mp h
+    obtain rfl := (Set.Finite.mem_toFinset _).mp hy
+    exact Finset.mem_singleton_self _
+  · intro hy; obtain rfl := Finset.mem_singleton.mp hy
+    refine Finset.mem_filter.mpr ⟨?_, ?_, ?_⟩ <;>
+      try (apply (Set.Finite.mem_toFinset _).mpr; exact Set.mem_singleton _)
+    · rintro _ ⟨⟩
+
+lemma singleton_erase {l : Type} [Bot l] (x : Node) (ℓ : l) :
+    (singleton x ℓ).nodes_finset.erase x = ∅ := by
+  apply Finset.eq_empty_of_forall_notMem; intro y hy
+  have ⟨hne, hy⟩ := Finset.mem_erase.mp hy
+  obtain rfl := (Set.Finite.mem_toFinset _).mp hy
+  contradiction
+
+lemma singleton_filter {l : Type} [Bot l] (x : Node) (ℓ : l) (r : Bool) :
+    (singleton x ℓ).filter_by_outcome (singleton x ℓ).nodes_finset x r = ∅ := by
+  apply Finset.eq_empty_of_forall_notMem; intro y hy
+  classical
+  have ⟨he, _⟩ := Finset.mem_filter.mp hy
+  rw [singleton_erase] at he; contradiction
+
+lemma lin_rec_eq_empty {t : Type → Type} {s act test : Type}
+    [Linearizable t s] [Bot (t s)]
+    [Sem act s (t s)] [Sem test s (t Bool)]
+    (α : Lpofin (Label act test)) {u : Finset Node}
+    (h : u = ∅) :
+    (α.lin_rec u : s → t s) = pure := by
+  ext σ; unfold lin_rec; refine if_pos h
+
+theorem lin_singleton {t : Type → Type} {s act test : Type}
+    [Linearizable t s] [Bot (t s)]
+    [Sem act s (t s)] [Sem test s (t Bool)]
+    (x : Node) (ℓ : Label act test) :
+    (lin (singleton x ℓ) : s → t s) = ℓ.eval := by
+  ext σ; unfold lin lin_rec
+  -- First iteration, node x gets evaluated
+  refine (if_neg ?_).trans ?_
+  · refine Finset.ne_empty_of_mem (a := x) ?_
+    exact (Set.Finite.mem_toFinset _).mpr (Set.mem_singleton _)
+  · conv => lhs; exact Nondet.finset_singleton x (singleton_next x ℓ)
+    simp only [lin_node, Label.eval]
+    have hℓ : (singleton x ℓ).lab x = ℓ := if_pos rfl; rw [hℓ]
+    cases ℓ with
+    | bot => rfl
+    | fork =>
+      exact congrFun (lin_rec_eq_empty _ (singleton_erase _ _)) _
+    | act a =>
+      refine Eq.trans ?_ (bind_pure _)
+      refine congrArg₂ Bind.bind rfl (lin_rec_eq_empty _ ?_)
+      exact singleton_erase _ _
+    | test b =>
+      simp only
+      rw [seqRight_eq_bind]; refine congrArg₂ Bind.bind rfl ?_
+      ext r; refine congrFun (lin_rec_eq_empty _ ?_) _
+      exact singleton_filter _ _ _
+
+end Lpofin
+
+
+namespace Pom
+
+theorem lin_singleton {t : Type → Type} {s act test : Type}
+    [Linearizable t s]
+    [∀ {β : Type}, OmegaCompletePartialOrder (t β)] [∀ {β : Type}, OrderBot (t β)]
+    [DCPO act] [Sem act s (t s)]
+    [DCPO test] [Sem test s (t Bool)]
+    (ℓ : Label act test) :
+    (lin (singleton ℓ) : s → t s) = ℓ.eval := by
+  rw [Pomfin.singleton_eq, lin_eq_fin]
+  conv => lhs; exact Pomfin.lin_mk _
+  exact Lpofin.lin_singleton default ℓ
+
+lemma lin_bot {t : Type → Type} {s act test : Type}
+    [Linearizable t s]
+    [∀ {β : Type}, OmegaCompletePartialOrder (t β)] [∀ {β : Type}, OrderBot (t β)]
+    [DCPO act] [Sem act s (t s)]
+    [DCPO test] [Sem test s (t Bool)] :
+    @lin t s act test _ _ _ _ _ _ _ (singleton ⊥) = ⊥ := lin_singleton _
+
+lemma lin_fork {t : Type → Type} {s act test : Type}
+    [Linearizable t s]
+    [∀ {β : Type}, OmegaCompletePartialOrder (t β)] [∀ {β : Type}, OrderBot (t β)]
+    [DCPO act] [Sem act s (t s)]
+    [DCPO test] [Sem test s (t Bool)] :
+    @lin t s act test _ _ _ _ _ _ _ (singleton Label.fork) = pure := lin_singleton _
+
+lemma lin_act {t : Type → Type} {s act test : Type}
+    [Linearizable t s]
+    [∀ {β : Type}, OmegaCompletePartialOrder (t β)] [∀ {β : Type}, OrderBot (t β)]
+    [DCPO act] [Sem act s (t s)]
+    [DCPO test] [Sem test s (t Bool)]
+    (a : act) :
+    @lin t s act test _ _ _ _ _ _ _ (singleton (Label.act a)) = Sem.sem a := lin_singleton _
+
+end Pom
